examples/n_german/n_mutualEx_base.thy
@@ -1,0 +1,462 @@
+(*  Title:      HOL/Auth/n_mutualEx_base.thy
+    Author:     Yongjian Li and Kaiqiang Duan, State Key Lab of Computer Science, Institute of Software, Chinese Academy of Sciences
+    Copyright    2016 State Key Lab of Computer Science, Institute of Software, Chinese Academy of Sciences
+*)
+
+(*header{*The n_mutualEx Protocol Case Study*} *)
+
+theory n_mutualEx_base imports paraTheoryCmpzb
+begin
+
+section{*Main definitions*}
+
+subsection{* Definitions of Constants*}
+definition I::"scalrValueType" where [simp]: "I\<equiv> enum ''control'' ''I''"
+definition T::"scalrValueType" where [simp]: "T\<equiv> enum ''control'' ''T''"
+definition C::"scalrValueType" where [simp]: "C\<equiv> enum ''control'' ''C''"
+definition E::"scalrValueType" where [simp]: "E\<equiv> enum ''control'' ''E''"
+definition true::"scalrValueType" where [simp]: "true\<equiv> boolV True"
+definition false::"scalrValueType" where [simp]: "false\<equiv> boolV False"
+
+
+
+subsection{*  Definitions of Parameterized Rules *}
+
+definition  NC::"nat " where [simp]: "NC==1"
+
+ definition VF::"varType set" where [simp]: 
+"VF \<equiv>{(Para ( ''n'') 0),(Para ( ''n'') 1),(Ident ''x'')}"
+definition n_Try::"nat \<Rightarrow> rule" where [simp]:
+"n_Try  i\<equiv>
+let g = (eqn (IVar (Para ( ''n'') i)) (Const I)) in
+let s = (parallelList [(assign ((Para ( ''n'') i), (Const T)))]) in
+guard g s"
+
+definition n_Crit::"nat \<Rightarrow> rule" where [simp]:
+"n_Crit  i\<equiv>
+let g = (andForm (eqn (IVar (Para ( ''n'') i)) (Const T)) (eqn (IVar (Ident ''x'')) (Const true))) in
+let s = (parallelList [(assign ((Para ( ''n'') i), (Const C))), (assign ((Ident ''x''), (Const false)))]) in
+guard g s"
+
+definition n_Exit::"nat \<Rightarrow> rule" where [simp]:
+"n_Exit  i\<equiv>
+let g = (eqn (IVar (Para ( ''n'') i)) (Const C)) in
+let s = (parallelList [(assign ((Para ( ''n'') i), (Const E)))]) in
+guard g s"
+
+definition n_Idle::"nat \<Rightarrow> rule" where [simp]:
+"n_Idle  i\<equiv>
+let g = (eqn (IVar (Para ( ''n'') i)) (Const E)) in
+let s = (parallelList [(assign ((Para ( ''n'') i), (Const I))), (assign ((Ident ''x''), (Const true)))]) in
+guard g s"
+
+definition n_Crit_i_3::"rule" where [simp]:
+"n_Crit_i_3  \<equiv>
+let g = (eqn (IVar (Ident ''x'')) (Const true)) in
+let s = (parallelList [(assign ((Ident ''x''), (Const false)))]) in
+guard g s"
+
+definition n_Idle_i_3::"rule" where [simp]:
+"n_Idle_i_3  \<equiv>
+let g = (andForm (andForm (eqn (IVar (Ident ''x'')) (Const false)) 
+(forallForm (down NC) (\<lambda>j. (neg (eqn (IVar (Para ( ''n'') j)) (Const E))))))
+ (forallForm (down NC) (\<lambda>j. (neg (eqn (IVar (Para ( ''n'') j)) (Const C)))))) in
+let s = (parallelList [(assign ((Ident ''x''), (Const true)))]) in
+guard g s"
+
+definition n_Idle_i_3PP::"nat \<Rightarrow> rule" where [simp]:
+"n_Idle_i_3PP i \<equiv>
+let g = andForm (eqn (IVar (Para ( ''n'') i)) (Const E)) (andForm (andForm (eqn (IVar (Ident ''x'')) (Const false)) 
+(forallForm (down NC) (\<lambda>j. (neg (eqn (IVar (Para ( ''n'') j)) (Const E))))))
+ (forallForm (down NC) (\<lambda>j. (neg (eqn (IVar (Para ( ''n'') j)) (Const C)))))) in
+let s = (parallelList [(assign ((Ident ''x''), (Const true)))]) in
+guard g s"
+
+subsection{*The set of All actual Rules w.r.t. a Protocol Instance with Size $N$*}
+definition rules::"nat \<Rightarrow> rule set" where [simp]:
+"rules N \<equiv> {r.
+(\<exists> i. i\<le>N\<and>r=n_Try  i) \<or>
+(\<exists> i. i\<le>N\<and>r=n_Crit  i) \<or>
+(\<exists> i. i\<le>N\<and>r=n_Exit  i) \<or>
+(\<exists> i. i\<le>N\<and>r=n_Idle  i) \<or>
+(r=n_Crit_i_3  ) \<or>
+(r=n_Idle_i_3  )\<or> r=skipRule
+}"
+
+
+
+subsection{*Definitions of a Formally Parameterized Invariant Formulas*}
+
+definition inv_27::"nat \<Rightarrow> formula" where [simp]:
+"inv_27 i \<equiv>
+(implyForm (eqn (IVar (Para ( ''n'') i)) (Const E)) (eqn (IVar (Ident ''x'')) (Const false)))"
+
+definition inv_7::"nat \<Rightarrow> nat \<Rightarrow> formula" where [simp]:
+"inv_7 i j \<equiv>
+(implyForm (neg (eqn (Const (index i)) (Const (index j)))) (implyForm (eqn (IVar (Para ( ''n'') i)) (Const E)) (neg (eqn (IVar (Para ( ''n'') j)) (Const E)))))"
+
+definition inv_5::"nat \<Rightarrow> nat \<Rightarrow> formula" where [simp]:
+"inv_5 i j \<equiv>
+(implyForm (neg (eqn (Const (index i)) (Const (index j)))) (implyForm (eqn (IVar (Para ( ''n'') i)) (Const E)) (neg (eqn (IVar (Para ( ''n'') j)) (Const C)))))"
+
+subsection{*Definitions of  the Set of Invariant Formula Instances in a $N$-protocol Instance*}
+definition invariants::"nat \<Rightarrow> formula set" where [simp]:
+"invariants N \<equiv> {f.
+(\<exists> i. i\<le>N\<and>f=inv_27  i) \<or>
+(\<exists> i j. i\<le>N\<and>j\<le>N\<and>i~=j\<and>f=inv_7  i j) \<or>
+(\<exists> i j. i\<le>N\<and>j\<le>N\<and>i~=j\<and>f=inv_5  i j)
+}" 
+
+subsection{*Definitions of  the Set of Abs Invariant Formula Instances *}
+definition invariantsAbs  ::"  formula list" where [simp]:
+"invariantsAbs   \<equiv> [
+inv_27 0 ,
+inv_7 0 1 ,
+inv_7 1 0 ,
+inv_5 0 1 ,
+inv_5 1 0
+]"
+
+definition initSpec0::"nat \<Rightarrow> formula" where [simp]:
+"initSpec0 N \<equiv> (forallForm (down N) (% i . (eqn (IVar (Para ( ''n'') i)) (Const I))))"
+
+definition initSpec1::"formula" where [simp]:
+"initSpec1  \<equiv> (eqn (IVar (Ident ''x'')) (Const true))"
+
+definition allInitSpecs::"nat \<Rightarrow> formula list" where [simp]:
+"allInitSpecs N \<equiv> [
+(initSpec0 N),
+(initSpec1 )
+]"
+axiomatization  where axiomOnf2 [simp,intro]:
+   "s ∈ reachableSet (set (allInitSpecs N )) (rules N) ⟹  1 < N ⟹ 1 < i ⟹ j<2 ⟹  formEval (f 0 1) s ⟹ formEval (f i j) s"
+
+axiomatization  where axiomOnf1 [simp,intro]:
+   "s ∈ reachableSet (set (allInitSpecs N )) (rules N) ⟹ 1 < N ⟹ 1 < i ⟹formEval (f 0 ) s ⟹ formEval (f i) s"
+
+
+
+
+subsection{*Definitions of initial states*}
+
+lemma lemmaOnn_TryGt_i:
+  assumes a1:"NC<i" and a2:"s ∈ reachableSet (set (allInitSpecs N)) (rules N)"  and  
+  a4:"∀f.  f ∈(set invariantsAbs) ⟶  formEval f s" 
+shows "trans_sim_on2 (n_Try  i  ) skipRule VF (set invariantsAbs) s" (is "trans_sim_on2 ?r ?r' VF ?F s")
+proof(unfold trans_sim_on2_def,(rule allI)+,(rule impI)+,rule disjI2)
+  fix s2 
+  assume b0:"state_sim_on2 s s2 VF "
+  show "state_sim_on2 (trans (act (n_Try  i)) s) s2  VF"
+  proof(cut_tac a1,unfold state_sim_on2_def,
+    (rule allI)+,(rule impI)+)
+    fix f v
+    assume b1:" v ∈  VF"  
+    
+    have b5:"trans (act (n_Try  i)) s v = s v" 
+      by (cut_tac a1  b1,auto) 
+
+    have b6:"s v =s2 v "
+      using b0 b1 state_sim_on2_def by blast  
+    show "trans (act (n_Try  i)) s v= s2 v"
+      using b5 b6 by auto 
+  qed
+qed
+lemma lemmaOnn_TryLeNc_:
+  assumes a1:"i\<le>NC" 
+  shows "trans_sim_on2 (n_Try  i) (n_Try  i) VF  (set invariantsAbs) s" (is "trans_sim_on2 ?r ?r VF ?F s")
+proof(rule ruleSimId2)
+  show  "∀v. v∈varOfForm (pre ?r) ⟶  v ∈ VF "
+    by(cut_tac a1, auto) 
+    
+next
+  show  b1: "∀v a. a ∈ set (statement2Assigns (act ?r)) ⟶ v∈varOfExp ( substExpByStatement (IVar (fst a))  (act ?r))⟶v ∈VF "
+   proof(cut_tac a1,(rule allI)+,(rule impI)+,auto) qed
+    
+ qed
+lemma lemmaOnn_Try: 
+  assumes   a2:"s ∈ reachableSet (set (allInitSpecs N)) (rules N)"  and  
+  a4:"∀f.  f ∈(set invariantsAbs) ⟶  formEval f s" and a5:"\<exists> i. i\<le>N\<and>r=n_Try  i"  and
+  a6:"NC<N"
+  shows "∃ r'. r' ∈ rules NC∧ trans_sim_on2 r r' VF (set invariantsAbs) s" (is "∃r'.?P1 r' ∧ ?P2 r'")
+proof -
+  from a5 obtain i where d0:"i\<le>N\<and>r=n_Try  i"  by blast
+  have "i>NC|i\<le> NC" by auto
+  moreover{
+       assume a1:"i>NC" 
+        have "∃r'. ?P1 r' ∧ ?P2 r'"
+        proof(rule_tac x="(skipRule)" in exI,rule conjI)
+          show  "?P1 (skipRule) " 
+           by(cut_tac a1, auto) 
+          next
+          show  "?P2 (skipRule) "
+           using lemmaOnn_TryGt_i local.a1 a2 a4 a6 d0 by blast 
+        qed
+       }
+moreover{
+       assume a1:"i\<le> NC" 
+        have "∃r'. ?P1 r' ∧ ?P2 r'"
+        proof(rule_tac x="(n_Try  i)" in exI,rule conjI)
+          show  "?P1 (n_Try  i) " 
+           by(cut_tac a1, auto) 
+          next
+          show  "?P2 (n_Try  i) "
+           using lemmaOnn_TryLeNc_ local.a1 a2 a4 a6 d0 by blast 
+        qed
+       }
+  ultimately show "∃r'.?P1 r' ∧ ?P2 r'" 
+    by satx
+qed
+
+lemma lemmaOnn_CritGt_i:
+  assumes a1:"i>NC" and 
+  a2:"s ∈ reachableSet (set (allInitSpecs N)) (rules N)"  and a3:"NC<N" and  
+  a4:"∀f.  f ∈(set invariantsAbs) ⟶  formEval f s" 
+  shows "trans_sim_on2 (n_Crit  i)  (n_Crit_i_3 ) VF (set invariantsAbs) s" (is "trans_sim_on2 ?r ?r' VF (set ?F) s")
+  proof(rule ruleSimCond2)
+    show " formEval (pre ?r) s ⟶formEval (pre ?r') s" (is "?A ⟶?B")
+    proof(rule impI)+
+      assume b0:"?A"
+  
+      from b0  show "formEval (pre ?r') s" 
+       by auto
+     qed
+   next 
+	show "(∀  v. v ∈  varOfSent (act  ?r') ⟶  v ∈ VF ⟶ formEval (pre ?r) s ⟶ 
+    expEval (substExpByStatement (IVar v)  (act ?r')) s = expEval (substExpByStatement (IVar v)  (act ?r)) s)"
+   proof(rule allI,(rule impI)+)
+      fix  v
+     assume b1:"v∈ VF"  and b2:"formEval (pre ?r) s" and b3:"v ∈varOfSent (act ?r')"
+  
+  show "expEval (substExpByStatement (IVar v)  (act ?r')) s = expEval (substExpByStatement (IVar v)  (act ?r)) s"  
+       apply (cut_tac  a1 b1 b2 ,auto) done
+   qed
+ next
+   show "∀  v. v ∈  varOfSent (act ?r) ⟶  v ∈ VF ⟶ v ∈  varOfSent (act ?r')" by(cut_tac a1, auto)
+
+  
+ next 
+   show "∀ v va. v ∈ varOfSent (act ?r') ⟶va∈varOfExp ( substExpByStatement (IVar v)  (act ?r'))⟶ va ∈ VF "
+     by auto  
+ next
+   show "∀v. v ∈ varOfForm (pre (?r')) ⟶ v ∈ VF" by auto
+qed
+lemma lemmaOnn_CritLeNc_:
+  assumes a1:"i\<le>NC" 
+  shows "trans_sim_on2 (n_Crit  i) (n_Crit  i) VF  (set invariantsAbs) s" (is "trans_sim_on2 ?r ?r VF ?F s")
+proof(rule ruleSimId2)
+  show  "∀v. v∈varOfForm (pre ?r) ⟶  v ∈ VF "
+    by(cut_tac a1, auto) 
+    
+next
+  show  b1: "∀v a. a ∈ set (statement2Assigns (act ?r)) ⟶ v∈varOfExp ( substExpByStatement (IVar (fst a))  (act ?r))⟶v ∈VF "
+   proof(cut_tac a1,(rule allI)+,(rule impI)+,auto) qed
+    
+ qed
+lemma lemmaOnn_Crit: 
+  assumes   a2:"s ∈ reachableSet (set (allInitSpecs N)) (rules N)"  and  
+  a4:"∀f.  f ∈(set invariantsAbs) ⟶  formEval f s" and a5:"\<exists> i. i\<le>N\<and>r=n_Crit  i"  and
+  a6:"NC<N"
+  shows "∃ r'. r' ∈ rules NC∧ trans_sim_on2 r r' VF (set invariantsAbs) s" (is "∃r'.?P1 r' ∧ ?P2 r'")
+proof -
+  from a5 obtain i where d0:"i\<le>N\<and>r=n_Crit  i"  by blast
+  have "i>NC|i\<le> NC" by auto
+  moreover{
+       assume a1:"i>NC" 
+        have "∃r'. ?P1 r' ∧ ?P2 r'"
+        proof(rule_tac x="(n_Crit_i_3 )" in exI,rule conjI)
+          show  "?P1 (n_Crit_i_3 ) " 
+           by(cut_tac a1, auto) 
+          next
+          show  "?P2 (n_Crit_i_3 ) "
+           using lemmaOnn_CritGt_i local.a1 a2 a4 a6 d0 by blast 
+        qed
+       }
+moreover{
+       assume a1:"i\<le> NC" 
+        have "∃r'. ?P1 r' ∧ ?P2 r'"
+        proof(rule_tac x="(n_Crit  i)" in exI,rule conjI)
+          show  "?P1 (n_Crit  i) " 
+           by(cut_tac a1, auto) 
+          next
+          show  "?P2 (n_Crit  i) "
+           using lemmaOnn_CritLeNc_ local.a1 a2 a4 a6 d0 by blast 
+        qed
+       }
+  ultimately show "∃r'.?P1 r' ∧ ?P2 r'" 
+    by satx
+qed
+
+lemma lemmaOnn_ExitGt_i:
+  assumes a1:"NC<i" and a2:"s ∈ reachableSet (set (allInitSpecs N)) (rules N)"  and  
+  a4:"∀f.  f ∈(set invariantsAbs) ⟶  formEval f s" 
+shows "trans_sim_on2 (n_Exit  i  ) skipRule VF (set invariantsAbs) s" (is "trans_sim_on2 ?r ?r' VF ?F s")
+proof(unfold trans_sim_on2_def,(rule allI)+,(rule impI)+,rule disjI2)
+  fix s2 
+  assume b0:"state_sim_on2 s s2 VF "
+  show "state_sim_on2 (trans (act (n_Exit  i)) s) s2  VF"
+  proof(cut_tac a1,unfold state_sim_on2_def,
+    (rule allI)+,(rule impI)+)
+    fix f v
+    assume b1:" v ∈  VF"  
+    
+    have b5:"trans (act (n_Exit  i)) s v = s v" 
+      by (cut_tac a1  b1,auto) 
+
+    have b6:"s v =s2 v "
+      using b0 b1 state_sim_on2_def by blast  
+    show "trans (act (n_Exit  i)) s v= s2 v"
+      using b5 b6 by auto 
+  qed
+qed
+lemma lemmaOnn_ExitLeNc_:
+  assumes a1:"i\<le>NC" 
+  shows "trans_sim_on2 (n_Exit  i) (n_Exit  i) VF  (set invariantsAbs) s" (is "trans_sim_on2 ?r ?r VF ?F s")
+proof(rule ruleSimId2)
+  show  "∀v. v∈varOfForm (pre ?r) ⟶  v ∈ VF "
+    by(cut_tac a1, auto) 
+    
+next
+  show  b1: "∀v a. a ∈ set (statement2Assigns (act ?r)) ⟶ v∈varOfExp ( substExpByStatement (IVar (fst a))  (act ?r))⟶v ∈VF "
+   proof(cut_tac a1,(rule allI)+,(rule impI)+,auto) qed
+    
+ qed
+lemma lemmaOnn_Exit: 
+  assumes   a2:"s ∈ reachableSet (set (allInitSpecs N)) (rules N)"  and  
+  a4:"∀f.  f ∈(set invariantsAbs) ⟶  formEval f s" and a5:"\<exists> i. i\<le>N\<and>r=n_Exit  i"  and
+  a6:"NC<N"
+  shows "∃ r'. r' ∈ rules NC∧ trans_sim_on2 r r' VF (set invariantsAbs) s" (is "∃r'.?P1 r' ∧ ?P2 r'")
+proof -
+  from a5 obtain i where d0:"i\<le>N\<and>r=n_Exit  i"  by blast
+  have "i>NC|i\<le> NC" by auto
+  moreover{
+       assume a1:"i>NC" 
+        have "∃r'. ?P1 r' ∧ ?P2 r'"
+        proof(rule_tac x="(skipRule)" in exI,rule conjI)
+          show  "?P1 (skipRule) " 
+           by(cut_tac a1, auto) 
+          next
+          show  "?P2 (skipRule) "
+           using lemmaOnn_ExitGt_i local.a1 a2 a4 a6 d0 by blast 
+        qed
+       }
+moreover{
+       assume a1:"i\<le> NC" 
+        have "∃r'. ?P1 r' ∧ ?P2 r'"
+        proof(rule_tac x="(n_Exit  i)" in exI,rule conjI)
+          show  "?P1 (n_Exit  i) " 
+           by(cut_tac a1, auto) 
+          next
+          show  "?P2 (n_Exit  i) "
+           using lemmaOnn_ExitLeNc_ local.a1 a2 a4 a6 d0 by blast 
+        qed
+       }
+  ultimately show "∃r'.?P1 r' ∧ ?P2 r'" 
+    by satx
+qed
+
+lemma lemmaOnn_IdleGt_i:
+  assumes a1:"i>NC" and 
+  a2:"s ∈ reachableSet (set (allInitSpecs N)) (rules N)"  and a3:"NC<N" and  
+  a4:"∀f.  f ∈(set invariantsAbs) ⟶  formEval f s" 
+  shows "trans_sim_on2 (n_Idle  i)  (n_Idle_i_3 ) VF (set invariantsAbs) s" (is "trans_sim_on2 ?r ?r' VF (set ?F) s")
+  proof(rule ruleSimCond2)
+    show " formEval (pre ?r) s ⟶formEval (pre ?r') s" (is "?A ⟶?B")
+    proof(rule impI)+
+      assume b0:"?A"
+  from a4  have tmp:"formEval (inv_27 0)  s"   
+            by (force simp del:inv_27_def) 
+        have tmp1:"formEval (inv_27 i  ) s" 
+        proof(cut_tac a1 a2 a3 tmp,rule axiomOnf1,force+)qed
+        with b0 a1 have c0:"formEval  (conclude (inv_27 i)) s" by auto
+from a4  have tmp:"formEval (inv_7 0 1)  s"   
+            by (force simp del:inv_7_def) 
+        have tmp1:"formEval (inv_7 i 0  ) s" 
+        proof(cut_tac a1 a2 a3 tmp,rule axiomOnf2,force+)qed
+        with b0 a1 have c1:"formEval  (conclude (inv_7 i 0)) s" by auto
+from a4  have tmp:"formEval (inv_7 0 1)  s"   
+            by (force simp del:inv_7_def) 
+        have tmp1:"formEval (inv_7 i 1  ) s" 
+        proof(cut_tac a1 a2 a3 tmp,rule axiomOnf2,force+)qed
+        with b0 a1 have c2:"formEval  (conclude (inv_7 i 1)) s" by auto
+from a4  have tmp:"formEval (inv_5 0 1)  s"   
+            by (force simp del:inv_5_def) 
+        have tmp1:"formEval (inv_5 i 0  ) s" 
+        proof(cut_tac a1 a2 a3 tmp,rule axiomOnf2,force+)qed
+        with b0 a1 have c3:"formEval  (conclude (inv_5 i 0)) s" by auto
+from a4  have tmp:"formEval (inv_5 0 1)  s"   
+            by (force simp del:inv_5_def) 
+        have tmp1:"formEval (inv_5 i 1  ) s" 
+        proof(cut_tac a1 a2 a3 tmp,rule axiomOnf2,force+)qed
+        with b0 a1 have c4:"formEval  (conclude (inv_5 i 1)) s" by auto
+
+      from b0 c0 c1 c2 c3 c4 show "formEval (pre ?r') s" 
+       by auto
+     qed
+   next 
+	show "(∀  v. v ∈  varOfSent (act  ?r') ⟶  v ∈ VF ⟶ formEval (pre ?r) s ⟶ 
+    expEval (substExpByStatement (IVar v)  (act ?r')) s = expEval (substExpByStatement (IVar v)  (act ?r)) s)"
+   proof(rule allI,(rule impI)+)
+      fix  v
+     assume b1:"v∈ VF"  and b2:"formEval (pre ?r) s" and b3:"v ∈varOfSent (act ?r')"
+  
+  show "expEval (substExpByStatement (IVar v)  (act ?r')) s = expEval (substExpByStatement (IVar v)  (act ?r)) s"  
+       apply (cut_tac  a1 b1 b2 ,auto) done
+   qed
+ next
+   show "∀  v. v ∈  varOfSent (act ?r) ⟶  v ∈ VF ⟶ v ∈  varOfSent (act ?r')" by(cut_tac a1, auto)
+
+  
+ next 
+   show "∀ v va. v ∈ varOfSent (act ?r') ⟶va∈varOfExp ( substExpByStatement (IVar v)  (act ?r'))⟶ va ∈ VF "
+     by auto  
+ next
+   show "∀v. v ∈ varOfForm (pre (?r')) ⟶ v ∈ VF" by auto
+qed
+lemma lemmaOnn_IdleLeNc_:
+  assumes a1:"i\<le>NC" 
+  shows "trans_sim_on2 (n_Idle  i) (n_Idle  i) VF  (set invariantsAbs) s" (is "trans_sim_on2 ?r ?r VF ?F s")
+proof(rule ruleSimId2)
+  show  "∀v. v∈varOfForm (pre ?r) ⟶  v ∈ VF "
+    by(cut_tac a1, auto) 
+    
+next
+  show  b1: "∀v a. a ∈ set (statement2Assigns (act ?r)) ⟶ v∈varOfExp ( substExpByStatement (IVar (fst a))  (act ?r))⟶v ∈VF "
+   proof(cut_tac a1,(rule allI)+,(rule impI)+,auto) qed
+    
+ qed
+lemma lemmaOnn_Idle: 
+  assumes   a2:"s ∈ reachableSet (set (allInitSpecs N)) (rules N)"  and  
+  a4:"∀f.  f ∈(set invariantsAbs) ⟶  formEval f s" and a5:"\<exists> i. i\<le>N\<and>r=n_Idle  i"  and
+  a6:"NC<N"
+  shows "∃ r'. r' ∈ rules NC∧ trans_sim_on2 r r' VF (set invariantsAbs) s" (is "∃r'.?P1 r' ∧ ?P2 r'")
+proof -
+  from a5 obtain i where d0:"i\<le>N\<and>r=n_Idle  i"  by blast
+  have "i>NC|i\<le> NC" by auto
+  moreover{
+       assume a1:"i>NC" 
+        have "∃r'. ?P1 r' ∧ ?P2 r'"
+        proof(rule_tac x="(n_Idle_i_3 )" in exI,rule conjI)
+          show  "?P1 (n_Idle_i_3 ) " 
+           by(cut_tac a1, auto) 
+          next
+          show  "?P2 (n_Idle_i_3 ) "
+           using lemmaOnn_IdleGt_i local.a1 a2 a4 a6 d0 by blast 
+        qed
+       }
+moreover{
+       assume a1:"i\<le> NC" 
+        have "∃r'. ?P1 r' ∧ ?P2 r'"
+        proof(rule_tac x="(n_Idle  i)" in exI,rule conjI)
+          show  "?P1 (n_Idle  i) " 
+           by(cut_tac a1, auto) 
+          next
+          show  "?P2 (n_Idle  i) "
+           using lemmaOnn_IdleLeNc_ local.a1 a2 a4 a6 d0 by blast 
+        qed
+       }
+  ultimately show "∃r'.?P1 r' ∧ ?P2 r'" 
+    by satx
+qed
+
+
+end
